ConstrainedDecodingFormalization/Char.lean
@@ -1,0 +1,43 @@
+import Mathlib.Data.Finset.Basic
+import Mathlib.Data.Fintype.Basic
+import Mathlib.Data.Fintype.Sum
+import Mathlib.Data.FinEnum
+import Mathlib.Tactic.Linarith
+
+/-- Extend character alphabet with EOS symbol-/
+inductive ExtChar (α : Type u)
+| char : α → ExtChar α
+| eos  : ExtChar α
+deriving BEq, DecidableEq, Repr
+
+instance {α} : Coe (α) (ExtChar α) := ⟨fun a => ExtChar.char a⟩
+instance {α} [e: FinEnum α] : FinEnum (ExtChar α) where
+  card := FinEnum.card α + 1
+  equiv :=
+    let e := e.equiv
+    { toFun := fun x =>
+        match x with
+        | ExtChar.eos     => ⟨FinEnum.card α, Nat.lt_succ_self _⟩
+        | ExtChar.char a  => ⟨e a, Nat.lt_succ_of_lt (Fin.is_lt (e a))⟩
+      invFun := fun i =>
+        if h : i.val < FinEnum.card α then ExtChar.char (e.symm ⟨i.val, h⟩)
+        else ExtChar.eos
+      left_inv := by
+        intro x
+        cases x with
+        | eos =>
+          simp
+        | char a =>
+          simp
+      right_inv := by
+        intro ⟨i, hi⟩
+        by_cases h : i < FinEnum.card α
+        · simp [h]
+        · have : i = FinEnum.card α := by
+            linarith
+          subst this
+          simp
+      }
+  decEq := by infer_instance
+
+abbrev Ch := ExtChar
