ConstrainedDecodingFormalization/Vocabulary.lean
@@ -1,3 +1,5 @@
+import ConstrainedDecodingFormalization.Char
+
 class Vocabulary ( α: Type u ) ( β: Type v ) [ BEq α ] where
   flatten : β → List α
   embed: α → β
@@ -5,3 +7,17 @@ class Vocabulary ( α: Type u ) ( β: Type v ) [ BEq α ] where
   -- singleton assumption
   fe: ∀ a, flatten (embed a) = [a]
   empty: ∀ b, flatten b ≠ []
+
+instance { α β } [BEq α] [b: Vocabulary α β] : Vocabulary (Ch α) (Ch β) where
+  flatten := fun x => match x with
+    | ExtChar.char c => List.map ExtChar.char (b.flatten c)
+    | ExtChar.eos    => [ExtChar.eos]
+  embed := fun x => match x with
+    | ExtChar.char c => ExtChar.char (b.embed c)
+    | ExtChar.eos    => ExtChar.eos
+  fe := by
+    intro a
+    cases a <;> simp [Vocabulary.fe]
+  empty := by
+    intro b
+    cases b <;> simp [Vocabulary.empty]
